jelly_fish/spec/get.v
@@ -1,10 +1,10 @@
-From iris.algebra Require Import auth frac_auth gmap gset.
+From iris.algebra Require Import gmap gset excl_auth dfrac_agree.
+From iris.base_logic.lib Require Import invariants.
+From iris.program_logic Require Import atomic.
 From iris.heap_lang Require Import proofmode.
 
-From SkipList.lib Require Import arg_max.
-From SkipList.jelly_fish Require Import code.
-From SkipList.lib Require Import misc node_rep node_lt.
-From SkipList.jelly_fish.inv Require Import list_equiv lazy_inv skip_inv.
+From SkipList.lib Require Import zrange gmap_extra.
+From SkipList.jelly_fish Require Import code inv.
 From SkipList.jelly_fish.spec Require Import find.
 
 
@@ -16,172 +16,89 @@ Module GetSpec (Params: SKIP_LIST_PARAMS).
   Export Find.
 
   Section Proofs.
-    Context `{!heapGS Σ, !skipGS Σ, !lockG Σ}.
-    
-    Theorem findAll_spec (k lvl: Z) (head curr: node_rep) 
-      (M: gmap Z (argmax Z)) (bot: bot_gname) 
-      (Γ: sub_gname) (subs: list sub_gname) :
-      {{{ 
-        skip_list_equiv lvl head M 1 bot (Γ :: subs)
-        ∗
-        (⌜ curr = head ⌝ ∨ own (s_auth Γ) (◯ {[ curr ]}))
-        ∗
-        ⌜ node_key curr < k < INT_MAX ⌝
-      }}}
-        findAll (rep_to_node curr) #k #lvl #0
-      {{{ pred succ sub, RET ((rep_to_node pred), (rep_to_node succ));
-        skip_list_equiv lvl head M 1 bot (Γ :: subs)
-        ∗
-        ⌜ last (Γ :: subs) = Some sub ⌝
-        ∗
-        (own (s_auth sub) (◯ {[ succ ]}) ∨ ⌜ succ = tail ⌝)
-        ∗
-        ⌜ k ∈ dom M ↔ node_key succ = k ⌝
-      }}}.
+    Context `{!heapGS Σ, !skipG Σ} (N: namespace).
+
+    Definition opt_to_val (opt: option (Z * Z)) : val :=
+      match opt with
+      | None => NONEV
+      | Some vt => SOMEV (#vt.1, #vt.2)
+      end.
+
+    Theorem findAll_spec (k lvl: Z) (head curr: node_rep) (Γm: map_gname) (Γ: gmap Z inv_gname) :
+      node_key curr < k < INT_MAX →
+      0 ≤ lvl ≤ MAX_HEIGHT →
+      (⌜ curr = head ⌝ ∨ own (Γ !!! lvl).(auth_gname) (◯ {[curr]})) -∗
+      inv (skipN N) (skip_list_inv head Γm Γ) -∗
+      <<< ∀∀ (m: gmap Z (Z * Z)), map m Γm >>>
+        findAll (rep_to_node curr) #k #lvl @ ↑(skipN N)
+      <<< map m Γm, RET opt_to_val (m !! k) >>>.
     Proof.
-      iIntros (Φ) "(Hlist & Hown_curr & Hrange) HΦ".
-      iRevert (curr head lvl Γ subs) "Hlist Hown_curr Hrange HΦ".
-      iLöb as "IH".
-      iIntros (curr head lvl Γ subs) "Hlist #Hown_curr %Hrange HΦ".
-      wp_lam. wp_pures.
-      
-      destruct subs as [|γ subs].
-      + iDestruct "Hlist" as "(%Hlvl & (Hown_frag & #Hinv))"; rewrite Hlvl.
-        wp_apply (find_bot_spec with "[Hown_frag]").
-        { by iFrame "# ∗". }
-        iIntros (pred succ) "(Hown_frag & %Hpred_key & #Hown_succ & %Hkey_in_S)".
+      iIntros "%Hk %Hlvl Hcurr #Hinv %Φ"; iRevert (lvl curr Hk Hlvl) "Hcurr".
+      iLöb as "IH"; iIntros (lvl curr Hk Hlvl) "#Hcurr AU".
+      wp_lam. wp_let. wp_let.
 
-        wp_pures.
-        iModIntro; iApply "HΦ". 
-        by iFrame "# ∗".
-      + iDestruct "Hlist" as "(%Hlvl & #Hinv & Hmatch)".
-        wp_apply find_sub_spec.
-        { by iFrame "# ∗". }
-        iIntros (pred succ) "(%Hrange' & #Hown_pred & #Hown_succ & _)".
+      awp_apply (find_spec with "Hcurr Hinv"); first done; first done.
+      iApply (aacc_aupd with "AU"); first done.
+      iIntros (m) "(Hexcl◯ & Hvals)"; iAaccIntro with "Hexcl◯".
+      { do 2 (iIntros "?"; iModIntro; iFrame). }
+      iIntros (pred succ) "(Hexcl◯ & %Hnin & #Hpred & #Hsucc & %Hk' & Hlock)".
+      iDestruct "Hlock" as (γl l) "(#Hlock & #His_lock)".
 
-        wp_pures. case_bool_decide as Hcase; wp_if.
-        - exfalso; inversion Hcase; lia.
-        - wp_bind (BinOp _ _ _).
-          iInv (levelN lvl) as (M' S L) "(Hinv_sub & _)" "Hclose".
-          iDestruct "Hinv_sub" as "(>%Hperm & >%Hsort & >Hown_auth & >Hown_toks & Hlist)".
+      destruct (decide (k = node_key succ)) as [->|Hneq].
+      + iModIntro; iLeft; iFrame.
+        iIntros "AU"; iModIntro.
+        wp_pures; wp_lam; wp_pures.
+        case_bool_decide; last congruence.
+        wp_pures; wp_lam; wp_pures.
 
-          iDestruct "Hown_pred" as "[%Heq | #Hown_pred]".
-          * wp_op.            
-            iMod ("Hclose" with "[Hlist Hown_auth Hown_toks]") as "_".
-            { iNext; iExists M', S, L; by iFrame. }
+        wp_bind (Load _). iInv "Hinv" as "Hskip".
+        iDestruct "Hsucc" as "[->|Hsucc]"; first (rewrite /node_key/= in Hk; lia).
+        iDestruct (frag_has_val with "Hskip []") as "(>Hval & Hskip)"; first done.
+        { by iNext. }
 
-            iModIntro; wp_pures.
-            iApply ("IH" with "[$] [] [%]").
-            { by iLeft. }
-            { lia. }
-            iNext; iIntros (? ? ?) "(? & ? & ? & ?)".
-            iApply "HΦ". by iFrame "# ∗".
-          * iAssert ⌜ In pred L ⌝%I with "[Hown_auth]" as %Hin.
-            {
-              iDestruct (own_valid_2 with "Hown_auth Hown_pred") 
-                as %[Hvalid%gset_included]%auth_both_valid_discrete.
-              rewrite -elem_of_list_In Hperm elem_of_elements.
-              iPureIntro; set_solver.
-            }
+        clear dependent m; iMod "AU" as (m) "[(Hexcl◯ & Hvals●) [_ Hclose]]".
+        iDestruct "Hval" as (v) "(Hpt & Hval)".
+        iDestruct (own_valid_2 with "Hvals● Hval") 
+          as %[->%gmap_disj_included%map_singleton_subseteq_l]%auth_both_valid_discrete.
 
-            rewrite list_equiv_invert_L; last done.
-            iDestruct "Hlist" as (v γl l s succ') "(>%Hsucc'_range & Hpt & #Hs & #Hl & #Hlock & Hnode & _ & Himp)".
-            iDestruct "Hnode" as"(>Hauth_pred & >Htoks_pred)".
-
-            assert ({[ pred ]} = {[ pred ]} ⋅ {[ pred ]}) as -> by set_solver.
-            iDestruct "Hauth_pred" as "(Hauth_pred & Hauth_pred_dup)".
-            assert ({[ pred ]} = {[ pred ]} ⋅ {[ pred ]}) as <- by set_solver.
-
-            wp_op.
-            iPoseProof ("Himp" $! {[ val_v dummy_val ]} dummy_val with "[Hpt Hauth_pred_dup Htoks_pred]") as "Hlist".
-            { iFrame; rewrite elem_of_singleton //. }
-            iMod ("Hclose" with "[Hlist Hown_auth Hown_toks]") as "_".
-            { iNext; iExists M', S, L; by iFrame. }
-
-            iModIntro; wp_pures.
-            iApply ("IH" with "[$] [Hauth_pred] [%]").
-            { by iRight. }
-            { lia. }
-            iNext; iIntros (? ? ?) "(? & ? & ? & ?)".
-            iApply "HΦ". by iFrame "# ∗".
+        wp_load.
+        iDestruct ("Hclose" with "[$]") as ">HΦ"; last iModIntro.
+        iModIntro; iSplitL "Hskip Hpt Hval".
+        { iNext; iApply "Hskip"; iExists v; iFrame. }
+        by wp_let; wp_lam; wp_pures.
+      + destruct (decide (lvl = 0)) as [->|].
+        - iModIntro; iRight; iFrame.
+          iIntros "HΦ"; iModIntro.
+          wp_pures; wp_lam; wp_pures.
+          case_bool_decide; first congruence.
+          wp_pures; iModIntro. 
+          replace (m !! k) with (@None (Z * Z)); first done.
+          symmetry; by apply not_elem_of_dom, Hnin.
+        - iModIntro; iLeft; iFrame.
+          iIntros "AU"; iModIntro.
+          wp_pures; wp_lam; wp_pures.
+          do 2 (case_bool_decide; first congruence; wp_pures).
+          iDestruct (has_lower_frag with "Hinv Hpred") as ">Hpred'"; first lia.          
+          by iApply ("IH" with "[%] [%] Hpred'"); first lia; first lia.
     Qed.
-    
-    Theorem get_spec (p: loc) (k: Z) (M: gmap Z (argmax Z)) 
-      (bot: bot_gname) (subs: list sub_gname)
-      (Hrange: INT_MIN < k < INT_MAX) :
-      {{{ is_skip_list p M 1 bot subs }}}
-        get #p #k
-      {{{ v, RET v;
-        is_skip_list p M 1 bot subs ∗ ((⌜ v = NONEV ⌝ ∗ ⌜ M !! k = None ⌝) ∨
-        ∃ (t z: Z) (S: gset Z), ⌜ v = SOMEV (#z, #t) ⌝ ∗ ⌜ M !! k = Some (prodZ S t) ⌝ ∗ ⌜ z ∈ S ⌝)
-      }}}.
+
+    Theorem get_spec (p: loc) (Γm: map_gname)
+      (k: Z) (Hrange: INT_MIN < k < INT_MAX) :
+      map_inv N p Γm -∗
+      <<< ∀∀ (m: gmap Z (Z * Z)), map m Γm >>>
+        get #p #k @ ↑(skipN N)
+      <<< map m Γm, RET opt_to_val (m !! k) >>>.
     Proof.
-      iIntros (Φ) "H HΦ".
-      iDestruct "H" as (head) "(Hpt & %Hmin & Hlist)".
+      iIntros "#H %Φ AU".
+      iDestruct "H" as (head Γ) "(Hp & %Hmin & #Hinv)".
       wp_lam. wp_let. wp_load.
 
-      destruct subs as [|Γ subs]; first by iExFalso.
-      wp_apply (findAll_spec with "[Hlist]").
-      { iFrame. iSplit. by iLeft. iPureIntro; lia. }
-      iIntros (pred succ sub) "(Hlist & %Hlast & #Hown & %Hkey_in_dom)".
-      wp_pures. wp_lam. wp_pures.
-      
-      case_bool_decide as Hcase; wp_if.
-      + wp_lam. wp_pures.
-        rewrite skip_list_equiv_inv.
-        iDestruct "Hlist" as (sub') "(%Hlast' & (Hown_frag & #Hinv) & Himp)".
-        assert (sub = sub') as <- by congruence.
-
-        wp_bind (Load _).
-        iInv (levelN 0) as (? S L) "(Hinv_sub & >Hown_frac & >%Hequiv)" "Hclose".
-        iDestruct "Hinv_sub" as "(>%Hperm & >%Hsort & >Hown_auth & >Hown_toks & Hlist)".
-        iDestruct (own_valid_2 with "Hown_frac Hown_frag") 
-          as %->%frac_auth_agree_L.
-
-        iAssert ⌜ In succ L ⌝%I with "[Hown_auth]" as %Hsucc.
-        {
-          iDestruct "Hown" as "[Hown|%Hfalse]"; last first.
-          {
-            assert (k = node_key tail) as -> by congruence.
-            rewrite /tail/node_key/= in Hrange; lia.
-          }
-
-          iDestruct (own_valid_2 with "Hown_auth Hown") 
-            as %[Hvalid%gset_included]%auth_both_valid_discrete.
-          rewrite -elem_of_list_In Hperm elem_of_elements.
-          iPureIntro; set_solver.
-        }
-
-        rewrite list_equiv_invert_L; last done.
-        iDestruct "Hlist" as (v γl l s succ') "(_ & Hpt' & _ & _ & _ & Hnode & >%Hval & Himp')".
-        destruct Hval as [vs [Hsome Hin]].
-        
-        wp_load.
-        iPoseProof ("Himp'" $! vs v with "[Hpt' Hnode]") as "Hlist".
-        { by iFrame. }
-        rewrite /opt_map /opt_insert insert_id //.
-        iMod ("Hclose" with "[Hlist Hown_auth Hown_toks Hown_frac]") as "_".
-        { iNext; iExists M, S, L; by iFrame. }
-        iPoseProof ("Himp" with "[$]") as "Hlist".
-
-        iModIntro; wp_pures.
-        iModIntro; iApply "HΦ". 
-        iSplit.
-        { iExists head; by iFrame. }
-
-        iPureIntro; right.
-        exists (val_ts v), (val_v v), vs.
-        inversion Hcase; subst.
-        rewrite //.
-      + iModIntro; iApply "HΦ". 
-        iSplit. 
-        { iExists head; by iFrame. }
-        
-        iPureIntro; left.
-        split; first done.
-        rewrite -not_elem_of_dom. intros Hin. 
-        rewrite Hkey_in_dom in Hin. congruence.
+      awp_apply (findAll_spec with "[] Hinv"); 
+        first lia; first (pose HMAX_HEIGHT; lia); first by iLeft.
+      iApply (aacc_aupd with "AU"); first done.
+      iIntros (m) "Hmap"; iAaccIntro with "Hmap".
+      { do 2 (iIntros "?"; iModIntro; iFrame). }
+      iIntros. iModIntro; iRight; iFrame. by iIntros.
     Qed.
-
   End Proofs.
 End GetSpec.
