lib/arg_max.v
@@ -2,23 +2,24 @@ From stdpp Require Import gmap.
 From iris.algebra Require Export local_updates proofmode_classes.
 
 
-Section arg_max.
+Inductive argmax `{Countable A} :=
+| prodZ : gset A → Z → argmax
+| botZ : argmax.
+Global Arguments argmax _ {_ _}.
+
+Section cmra.
   Context `{Countable A}.
   Local Open Scope Z.
+  Local Arguments op _ _ !_ !_ /.
+  Local Arguments cmra_op _ !_ !_ /.
+  Local Arguments ucmra_op _ !_ !_ /.
 
-  Inductive argmax :=
-  | prodZ : gset A → Z → argmax
-  | botZ : argmax.
+  Canonical Structure argmax0 := leibnizO (argmax A).
 
-  Canonical Structure argmax0 := leibnizO argmax.
-
-  Definition args (p: argmax) : gset A :=
-    match p with
-    | prodZ a i => a
-    | botZ => ∅
-    end.
-
-  Definition arg_max (m n: argmax) : argmax :=
+  Local Instance arg_max_valid_instance : Valid (argmax A) := λ _, True.
+  Local Instance arg_max_unit_instance : Unit (argmax A) := botZ.
+  Local Instance arg_max_pcore_instance : PCore (argmax A) := Some.
+  Local Instance arg_max_op_instance : Op (argmax A) := λ n m,
     match m, n with
     | prodZ a i, prodZ b j => if (decide (i = j)) then prodZ (a ∪ b) i
                               else if (decide (i < j)) then n else m
@@ -26,77 +27,19 @@ Section arg_max.
     | _, botZ => m
     end.
 
-  Lemma arg_max_id :
-    ∀ m : argmax, arg_max m m = m.
-  Proof.
-    intros m.
-    destruct m as [a i|].
-    + rewrite /arg_max.
-      destruct (decide (i = i)); last done.
-      by assert (a ∪ a = a) as -> by set_solver.
-    + rewrite /arg_max //.
-  Qed.
-
-  Lemma arg_max_comm :
-    ∀ m n : argmax, arg_max m n = arg_max n m.
-  Proof.
-    intros m n.
-    destruct m as [a i|]; destruct n as [b j|]; rewrite /arg_max //.
-
-    destruct (decide (i = j)); simpl;
-    destruct (decide (j = i)); simpl;
-    try congruence; subst.
-    { rewrite comm_L //. }
-
-    destruct (decide (i < j));
-    destruct (decide (j < i));
-    try lia; done.
-  Qed.
-
-  Lemma arg_max_assoc :
-    ∀ m n p : argmax, arg_max m (arg_max n p) = arg_max (arg_max m n) p.
-  Proof.
-    intros m n p.
-    destruct m as [a i|]; 
-    destruct n as [b j|]; 
-    destruct p as [c k|]; 
-    rewrite /arg_max //.
-
-    + destruct (decide (j = k)) eqn: Hjk;
-      destruct (decide (i = j)) eqn:Hij; 
-      destruct (decide (i = k)) eqn:Hik;
-      try congruence;
-      destruct (decide (j < k)) eqn: Hjk';
-      destruct (decide (i < j)); 
-      destruct (decide (i < k));
-      try lia; 
-      rewrite ?Hjk ?Hij ?Hik ?Hjk' //.
-      rewrite assoc_L //.
-    + destruct (decide (i = j));
-      destruct (decide (i < j));
-      done.
-  Qed.
-End arg_max.
-Global Arguments argmax _ {_ _}.
-
-Section cmra.
-  Context `{Countable A}.
-  Local Open Scope Z.
-
-  Local Instance arg_max_unit_instance : Unit (argmax A) := botZ.
-  Local Instance arg_max_valid_instance : Valid (argmax A) := λ _, True.
-  Local Instance arg_max_validN_instance : ValidN (argmax A) := λ _ _, True.
-  Local Instance arg_max_pcore_instance : PCore (argmax A) := Some.
-  Local Instance arg_max_op_instance : Op (argmax A) := λ n m, arg_max n m.
-  Definition arg_max_op x y : x ⋅ y = arg_max x y := eq_refl.
+  Global Instance : IdemP (=@{argmax A}) (⋅).
+  Proof. intros [a i|]; rewrite ///op/arg_max_op_instance idemp_L; by case_decide. Qed.
 
   Lemma arg_max_ra_mixin : RAMixin (argmax A).
   Proof.
     apply ra_total_mixin; apply _ || eauto.
-    + intros x y z. repeat rewrite arg_max_op.
-      rewrite arg_max_assoc //.
-    + intros x y. by rewrite arg_max_op arg_max_comm.
-    + intros x. by rewrite arg_max_op arg_max_id.
+    + intros [a i|] [b j|] [c k|];
+        repeat rewrite ///op/arg_max_op_instance; repeat case_decide; try done; try lia.
+      rewrite assoc_L //.
+    + intros [a i|] [b j|]; 
+        repeat rewrite ///op/arg_max_op_instance; repeat case_decide; try done; try lia.
+      subst; rewrite comm_L //.
+    + intros x; rewrite idemp //.
   Qed.
   Canonical Structure arg_maxR : cmra := discreteR (argmax A) arg_max_ra_mixin.
 
@@ -104,61 +47,36 @@ Section cmra.
   Proof. apply discrete_cmra_discrete. Qed.
 
   Lemma arg_max_ucmra_mixin : UcmraMixin (argmax A).
-  Proof. split; try apply _ || done. Qed.
+  Proof. split; try apply _ || done. intros [x|]; done. Qed.
   Canonical Structure arg_maxUR : ucmra := Ucmra (argmax A) arg_max_ucmra_mixin.
 
   Global Instance arg_max_core_id (x : argmax A) : CoreId x.
   Proof. by constructor. Qed.
 
-  Lemma arg_max_included (x y: argmax A) : x ≼ y ↔ arg_max x y = y.
+  Lemma arg_max_included (x y: argmax A) : x ≼ y ↔ x ⋅ y = y.
   Proof.
-    split.
-    - intros [z ->].
-      rewrite arg_max_assoc arg_max_id //.
-    - by exists y.
+    split; last by exists y.
+    intros [z ->]; rewrite assoc idemp //.
   Qed.
 
   Lemma arg_max_lt (a b : gset A) (i j : Z)  :
     i < j → prodZ a i ⋅ prodZ b j = prodZ b j.
-  Proof.
-    intros. rewrite arg_max_op /arg_max.
-    destruct (decide (i = j)); first lia.
-    destruct (decide (i < j)); last lia.
-    done.
-  Qed.
-
+  Proof. intros; rewrite /op/arg_max_op_instance; repeat case_decide; try lia; done. Qed.
   Lemma arg_max_eq (a b : gset A) (i : Z) :
     prodZ a i ⋅ prodZ b i = prodZ (a ∪ b) i.
-  Proof.
-    rewrite arg_max_op /arg_max.
-    by destruct (decide (i = i)).
-  Qed.
-
+  Proof. rewrite comm_L /op/arg_max_op_instance; by case_decide. Qed.
   Lemma arg_max_bot (m : argmax A) :
     m ⋅ botZ = m.
-  Proof.
-    rewrite arg_max_op /arg_max.
-    by destruct m.
-  Qed.
-
-  Lemma arg_max_args (a b : gset A) (i j : Z) :
-    args (prodZ a i ⋅ prodZ b j) ⊆ a ∪ b.
-  Proof.
-    destruct (decide (i = j)) as [<-|]; first by rewrite arg_max_eq.
-    destruct (decide (i < j)); first (rewrite arg_max_lt //; apply union_subseteq_r).
-    assert (j < i) by lia; rewrite comm arg_max_lt //; apply union_subseteq_l.
-  Qed.
+  Proof. by destruct m. Qed.
 
   Lemma arg_max_local_update (x y z : argmax A) :
     (x,y) ~l~> (z ⋅ x,z ⋅ y).
   Proof. by apply op_local_update. Qed.
 
-  Global Instance : IdemP (=@{argmax A}) (⋅).
-  Proof. intros x. rewrite arg_max_op arg_max_id //. Qed.
-
   Global Instance arg_max_is_op (x y : argmax A) :
     IsOp (x ⋅ y) x y.
   Proof. done. Qed.
 End cmra.
+
 Global Arguments arg_maxR _ {_ _}.
 Global Arguments arg_maxUR _ {_ _}.
