jelly_fish/inv.v
@@ -1,0 +1,200 @@
+From iris.algebra Require Import gmap gset excl_auth dfrac_agree.
+From iris.base_logic.lib Require Import invariants.
+From iris.heap_lang Require Import proofmode.
+
+From SkipList.lib Require Import zrange gmap_extra.
+From SkipList.jelly_fish Require Import code.
+
+
+Class skipG Σ := SkipG { 
+  skip_authG :> inG Σ (authR (gsetR node_rep));
+  skip_disjG :> inG Σ (gset_disjR Z);
+  skip_toksG :> inG Σ (authR (gset_disjR Z));
+  skip_exclG :> inG Σ (excl_authR (gset Z));
+  skip_valsG :> inG Σ (authR (gmap_disjR Z (Z * Z)));
+  skip_lockG :> lockG Σ
+}.
+
+Record inv_gname := mk_inv_gname {
+  auth_gname: gname;
+  disj_gname: gname;
+  toks_gname: gname
+}.
+Global Instance inv_gname_inhabited : Inhabited inv_gname := 
+  populate (mk_inv_gname inhabitant inhabitant inhabitant).
+
+Record map_gname := mk_map_gname {
+  excl_gname: gname;
+  vals_gname: gname
+}.
+
+Module SkipListInv (Params: SKIP_LIST_PARAMS).
+  Import Params.
+  Module SkipList := SkipList Params.
+  Export SkipList.
+
+  Section invariant.
+    Context `{!heapGS Σ, !skipG Σ} (N: namespace).
+    Local Open Scope Z.
+
+    Definition locked_val (lvl: Z) (n: loc) : iProp Σ := 
+      if decide (lvl = 0) then 
+        (∃ (node: node_rep), n ↦□ rep_to_node node ∗
+        (⌜ node = tail ⌝ ∨ ∃ (val: val_rep), (node_val node) ↦{#1 / 2} rep_to_val val))%I
+      else True%I.
+    Definition in_lock (lvl: Z) (a: loc) : iProp Σ := 
+      ∃ (n: loc), (a +ₗ lvl) ↦{#1 / 2} #n ∗ locked_val lvl n.
+    Definition has_lock (lvl: Z) (node: node_rep) : iProp Σ := 
+      ∃ (γl: gname) (l: val), 
+        (node_lock node +ₗ lvl) ↦□ l
+        ∗
+        is_lock γl l (in_lock lvl (node_next node)).
+
+    Definition has_next (lvl: Z) (Γi: inv_gname) (pred: node_rep) : iProp Σ :=
+      ∃ (s: loc) (succ: node_rep), 
+        (node_next pred +ₗ lvl) ↦{#1 / 2} #s
+        ∗
+        s ↦□ rep_to_node succ
+        ∗
+        (⌜ succ = tail ⌝ ∨ own Γi.(auth_gname) (◯ {[succ]}))
+        ∗
+        own Γi.(disj_gname) (ZRange (node_key pred) (node_key succ)).
+
+    Definition has_val (Γm: map_gname) (node: node_rep) : iProp Σ :=
+      ∃ (val: val_rep),
+        (node_val node) ↦{#1 / 2} rep_to_val val
+        ∗
+        own Γm.(vals_gname) (◯ DMap {[ node_key node := (val_vt val)]}).
+    Definition own_map (S: gset node_rep) (Γm: map_gname) : iProp Σ :=
+      own Γm.(excl_gname) (●E (set_map node_key S))
+      ∗
+      [∗ set] n ∈ S, has_val Γm n.
+
+    Definition has_frag (γi: inv_gname) (node: node_rep) : iProp Σ :=
+      own γi.(auth_gname) (◯ {[ node ]})
+      ∗
+      own γi.(toks_gname) (◯ GSet {[ node_key node ]}).
+
+    Definition lazy_list_inv (head: node_rep) (Γm: map_gname) (Γ: gmap Z inv_gname) (lvl: Z) : iProp Σ :=
+      ∃ (S: gset node_rep),
+        own (Γ !!! lvl).(auth_gname) (● S)
+        ∗
+        own (Γ !!! lvl).(disj_gname) (GSet (set_map node_key S))
+        ∗
+        own (Γ !!! lvl).(toks_gname) (● GSet (set_map node_key S))
+        ∗
+        ([∗ set] n ∈ {[head]} ∪ S, has_lock lvl n)
+        ∗
+        ([∗ set] n ∈ {[head]} ∪ S, has_next lvl (Γ !!! lvl) n)
+        ∗
+        if decide (lvl = 0) then own_map S Γm
+        else [∗ set] n ∈ S, has_frag (Γ !!! (lvl - 1)) n.
+    Definition skip_list_inv (head: node_rep) (Γm: map_gname) (Γ: gmap Z inv_gname) : iProp Σ :=
+      [∗ set] i ∈ zrange (-1) (MAX_HEIGHT + 1), lazy_list_inv head Γm Γ i.
+
+    Definition skipN := N .@ "skip".
+    Definition map_inv (p: loc) (Γm: map_gname) : iProp Σ :=
+      ∃ (head: node_rep) (Γ: gmap Z inv_gname),
+        p ↦□ rep_to_node head
+        ∗
+        ⌜ node_key head = INT_MIN ⌝
+        ∗
+        inv skipN (skip_list_inv head Γm Γ).
+
+    Definition map (m: gmap Z (Z * Z)) (Γm: map_gname) : iProp Σ := 
+      own Γm.(excl_gname) (◯E (dom m))
+      ∗
+      own Γm.(vals_gname) (● DMap m).
+
+  End invariant.
+
+  Section proofs.
+    Context `{!heapGS Σ, !skipG Σ} (N: namespace).
+    Local Open Scope Z.
+
+    Lemma singleton_frag_in (S: gset node_rep) (n s: node_rep) (γ: gname) :
+      own γ (● S) -∗ ⌜ n = s ⌝ ∨ own γ (◯ {[n]}) → ⌜ n ∈ {[s]} ∪ S ⌝.
+    Proof.
+      iIntros "Hauth Hnode".
+      iDestruct "Hnode" as "[->|Hnode]"; first (iPureIntro; set_solver).
+      iDestruct (own_valid_2 with "Hauth Hnode") 
+        as %[?%gset_included]%auth_both_valid_discrete.
+      iPureIntro; set_solver.
+    Qed.
+
+    Lemma has_lvl_inv (lvl: Z) (head: node_rep) 
+      (Γm: map_gname) (Γ: gmap Z inv_gname) :
+      0 ≤ lvl ≤ MAX_HEIGHT →
+      skip_list_inv head Γm Γ ⊢
+        lazy_list_inv head Γm Γ lvl
+        ∗
+        (lazy_list_inv head Γm Γ lvl -∗ skip_list_inv head Γm Γ).
+    Proof.
+      intros Hlvl; unfold skip_list_inv.
+      rewrite (big_sepS_delete _ _ lvl); last (rewrite zrange_spec; lia).
+      iIntros "(Hlvl & Hskip)"; iFrame; by iIntros.
+    Qed.
+
+    Lemma frag_has_val (lvl: Z) (head node: node_rep) 
+      (Γm: map_gname) (Γ: gmap Z inv_gname) :
+      0 ≤ lvl ≤ MAX_HEIGHT →
+      skip_list_inv head Γm Γ -∗
+      own (Γ !!! lvl).(auth_gname) (◯ {[node]}) -∗
+          has_val Γm node
+          ∗
+          (has_val Γm node -∗ skip_list_inv head Γm Γ).
+    Proof.
+      iIntros (Hlvl) "Hskip Hnode".
+      assert (lvl = Z.of_nat (Z.to_nat lvl)) as Heq by lia.
+      iRevert (Hlvl) "Hnode"; rewrite Heq; clear Heq.
+      iInduction (Z.to_nat lvl) as [|lvl'] "Himp"; iIntros "%Hlvl Hnode".
+      + iDestruct (has_lvl_inv 0 with "Hskip") as "(Hlvl & Hskip)"; first (pose HMAX_HEIGHT; lia).
+        iDestruct "Hlvl" as (S) "(Hauth & ? & ? & ? & ? & Hmap)".
+        iDestruct (own_valid_2 with "Hauth Hnode") as %[?%gset_included]%auth_both_valid_discrete.
+        iDestruct "Hmap" as "(Hexcl● & Hvals◯)".
+        rewrite (big_sepS_delete (has_val _) _ node); last set_solver.
+        iDestruct "Hvals◯" as "(Hval & Hvals◯)"; iFrame.
+        iIntros "Hval"; iCombine "Hval Hvals◯" as "Hvals◯". 
+        rewrite -big_sepS_delete; last set_solver.
+        iApply "Hskip"; iExists S; iFrame.
+      + iDestruct (has_lvl_inv with "Hskip") as "(Hlvl & Hskip)"; first done.
+        iDestruct "Hlvl" as (S) "(Hauth & ? & ? & ? & ? & Hfrags)".
+        case_decide; first lia.
+        iDestruct (own_valid_2 with "Hauth Hnode") as %[?%gset_included]%auth_both_valid_discrete.
+        rewrite (big_sepS_delete (has_frag _) _ node); last set_solver.
+        iDestruct "Hfrags" as "((#Hnode' & ?) & Hfrags)".
+        iAssert (has_frag _ _) with "[$]" as "Hfrag".
+        iCombine "Hfrag Hfrags" as "Hfrags".
+        rewrite -(big_sepS_delete (has_frag _)); last set_solver.
+        replace (Z.of_nat lvl') with (Datatypes.S lvl' - 1) by lia.
+        iApply ("Himp" with "[-] [%] [$]"); last lia.
+        iApply "Hskip". iExists S; case_decide; first lia; iFrame.
+    Qed.
+
+    Lemma has_lower_frag (lvl: Z) (head node: node_rep) 
+      (Γm: map_gname) (Γ: gmap Z inv_gname) :
+      0 < lvl ≤ MAX_HEIGHT →
+      inv (skipN N) (skip_list_inv head Γm Γ) -∗
+      ⌜ node = head ⌝ ∨ own (auth_gname (Γ !!! lvl)) (◯ {[node]}) ={⊤}=∗
+      ⌜ node = head ⌝ ∨ own (auth_gname (Γ !!! (lvl - 1))) (◯ {[node]}).
+    Proof.
+      iIntros (Hlvl) "#Hinv Hnode".
+      iDestruct "Hnode" as "[->|Hnode]"; first by (iModIntro; iLeft).
+      iInv "Hinv" as "Hskip".
+      iDestruct (has_lvl_inv lvl with "Hskip") as "(Hlvl & Hskip)"; first lia.
+      iDestruct "Hlvl" as (S) "(>Hauth & ? & ? & ? & ? & Hfrags)".
+      case_decide; first lia; iMod "Hfrags".
+
+      iDestruct (own_valid_2 with "Hauth Hnode") 
+        as %[?%gset_included]%auth_both_valid_discrete.
+      rewrite (big_sepS_delete (has_frag _) _ node); last set_solver.
+      iDestruct "Hfrags" as "((#Hnode' & ?) & Hfrags)".
+      iAssert (has_frag _ _) with "[$]" as "Hfrag".
+      iCombine "Hfrag Hfrags" as "Hfrags".
+      rewrite -(big_sepS_delete (has_frag _)); last set_solver.
+
+      iModIntro; iSplitR ""; last (iModIntro; iFrame "Hnode'").
+      iNext; iApply "Hskip"; iExists S; case_decide; first lia; iFrame.
+    Qed.
+  End proofs.
+End SkipListInv.
