jelly_fish/spec/find.v
@@ -1,412 +1,206 @@
-From Coq Require Import Sorting.Sorted.
-
+From iris.algebra Require Import gmap gset excl_auth dfrac_agree.
 From iris.base_logic.lib Require Import invariants.
-From iris.algebra Require Import auth frac_auth gmap gset.
+From iris.program_logic Require Import atomic.
 From iris.heap_lang Require Import proofmode.
 
-From SkipList.lib Require Import arg_max.
-From SkipList.jelly_fish Require Import code.
-From SkipList.lib Require Import misc node_rep node_lt.
-From SkipList.jelly_fish.inv Require Import list_equiv lazy_inv skip_inv.
+From SkipList.lib Require Import zrange.
+From SkipList.jelly_fish Require Import code inv.
 
-
-Local Open Scope Z.
 
 Module FindSpec (Params: SKIP_LIST_PARAMS).
   Import Params.
   Module Invariant := SkipListInv Params.
   Export Invariant.
 
-  Section Proofs.
-    Context `{!heapGS Σ, !skipGS Σ, !lockG Σ}.
+  Section proofs.
+    Context `{!heapGS Σ, !skipG Σ} (N: namespace).
+    Local Open Scope Z.
     
-    Theorem find_bot_spec (k: Z) (head curr: node_rep) 
-      (M: gmap Z (argmax Z)) (bot: bot_gname) (sub: sub_gname) :
-      {{{ 
-        inv (levelN 0) (lazy_list_inv 0 head (Some bot) sub None)
+    Theorem find_spec (k lvl: Z) (head curr: node_rep) (Γm: map_gname) (Γ: gmap Z inv_gname) :
+      node_key curr < k < INT_MAX →
+      0 ≤ lvl ≤ MAX_HEIGHT →
+      (⌜ curr = head ⌝ ∨ own (Γ !!! lvl).(auth_gname) (◯ {[curr]})) -∗
+      inv (skipN N) (skip_list_inv head Γm Γ) -∗
+      <<< ∀∀ (s: gset Z), own Γm.(excl_gname) (◯E s) >>>
+        find (rep_to_node curr) #k #lvl @ ↑(skipN N)
+      <<< ∃∃ pred succ,
+        own Γm.(excl_gname) (◯E s)
         ∗
-        own (s_frac bot) (◯F M)
+        ⌜ k ≠ node_key succ → lvl = 0 → k ∉ s ⌝
         ∗
-        (⌜ curr = head ⌝ ∨ own (s_auth sub) (◯ {[ curr ]}))
+        (⌜ pred = head ⌝ ∨ own (Γ !!! lvl).(auth_gname) (◯ {[pred]}))
         ∗
-        ⌜ node_key curr < k < INT_MAX ⌝
-      }}}
-        find (rep_to_node curr) #k #0
-      {{{ pred succ, RET ((rep_to_node pred), (rep_to_node succ));
-        own (s_frac bot) (◯F M)
+        (⌜ succ = tail ⌝ ∨ own (Γ !!! lvl).(auth_gname) (◯ {[succ]}))
         ∗
-        ⌜ node_key pred < k ⌝
-        ∗
-        (own (s_auth sub) (◯ {[ succ ]}) ∨ ⌜ succ = tail ⌝)
-        ∗
-        ⌜ k ∈ dom M ↔ node_key succ = k ⌝
-      }}}.
-    Proof.
-      iIntros (Φ) "(#Hinv & Hown_frag & Hown_curr & Hrange) HΦ".
-      iRevert (curr) "Hown_frag Hown_curr Hrange HΦ".
-      iLöb as "IH".
-      iIntros (curr) "Hown_frac_frag #Hown_curr %Hrange HΦ".
-      wp_lam. wp_pures. 
-      wp_lam. wp_pures.
-
-      wp_bind (Load #(node_next curr +ₗ 0)).
-      iInv (levelN 0) as (? S L) "(Hinv_sub & >Hown_frac & >%Hequiv)" "Hclose".
-      iDestruct "Hinv_sub" as "(>%Hperm & >%Hsort & >Hown_auth & >Hown_toks & Hlist)".
-      iDestruct (own_valid_2 with "Hown_frac Hown_frac_frag") 
-        as %->%frac_auth_agree_L.
-
-      iMod (own_update with "Hown_auth") as "[Hown_auth Hown_frag]".
-      { by apply auth_update_alloc, (gset_local_update S _ S). }
-
-      iAssert ⌜ curr = head ∨ In curr L ⌝%I with "[Hown_auth Hown_curr]" as %Hcurr_range.
-      {
-        iDestruct "Hown_curr" as "[Heq|Hown]"; first by iLeft.
-        iDestruct (own_valid_2 with "Hown_auth Hown") 
-          as %[Hvalid%gset_included]%auth_both_valid_discrete.
-        iPureIntro; right.
-        rewrite -elem_of_list_In Hperm elem_of_elements.
-        set_solver.
-      }
-
-      edestruct (in_cons_split curr head L) 
-        as (Ls&Lf&(Hcurr&Hsub)).
-      { rewrite in_inv //. }
-
-      edestruct (node_rep_split_join Lf curr tail k) 
-        as (pred&succ&L1&L2&?&?&Hpred_range&Hsucc_range&Hsplit_join); auto.
-      {
-        rewrite /= app_comm_cons Hcurr app_ass in Hsort.
-        apply node_rep_sorted_app in Hsort.
-        simpl in *. by destruct Hsort as [_ ?].
-      }
-
-      feed pose proof (node_rep_split_sep L Ls Lf L1 L2 head curr pred succ tail k) 
-        as Htemp; auto.
-      destruct Htemp as [Lm Hsplit_sep].
-
-      destruct Lm as [|next Lm].
-      - rewrite list_equiv_split; last first.
-        { rewrite app_ass -Hsplit_sep //. }
-        iDestruct "Hlist" as (s) "(Hpt & #Hs & Himp)".
-
-        wp_load.
-        iPoseProof ("Himp" with "Hpt") as "Hlist".
-        iMod ("Hclose" with "[Hlist Hown_auth Hown_toks Hown_frac]") as "_".
-        { iNext; iExists M, S, L; by iFrame. }
-
-        iModIntro. wp_load. 
-        wp_let. wp_lam. wp_pures.
-        case_bool_decide; last lia.
-        wp_pures. iApply "HΦ".
-        iModIntro; iFrame "# ∗".
-
-        iSplit; first by (iPureIntro; lia).
-        iSplit.
-        { 
-          destruct Hsucc_range as [Hin|Heq]; last by iRight.
-          rewrite -elem_of_list_In in Hin.
-          rewrite Hperm in Hsub.
-          assert (S = S ⋅ {[ succ ]}) as -> by set_solver.
-          iDestruct "Hown_frag" as "(? & ?)"; iLeft; iFrame.
-        }
-
-        iPureIntro.
-        rewrite Hequiv elem_of_map.
-        split.
-        * intros [rep [Hkey HinS]].
-          rewrite -elem_of_elements -Hperm in HinS.
-          eapply (sorted_node_lt_cover_gap (Ls ++ L1) L2 pred); try lia.
-          ++ by rewrite app_ass -Hsplit_join //= app_comm_cons -app_ass -Hcurr -app_comm_cons.
-          ++ assert (In k (map node_key (head :: L ++ [tail]))) as Hin.
-             { 
-               right. 
-               rewrite map_app in_app_iff -elem_of_list_In.
-               left. rewrite elem_of_list_In in_map_iff.
-               exists rep. rewrite -elem_of_list_In //.
-             }        
-             rewrite app_comm_cons Hcurr app_ass in Hin.
-             by rewrite app_ass -Hsplit_join.
-        * intros; exists succ. split; first done.
-          rewrite -elem_of_elements -Hperm elem_of_list_In.
-
-          assert (In succ Lf).
-          { 
-            rewrite -in_inv_rev /tail ?in_app_iff in Hsucc_range.
-            destruct Hsucc_range as [|[|[]]]; auto; subst. 
-            rewrite /node_key /= in Hrange; lia. 
-          }
-
-          destruct Ls; inversion Hcurr; subst; auto.
-          intros; by rewrite in_app_iff; right; right.
-      - assert (next ∈ S).
-        {
-          rewrite -elem_of_elements -Hperm elem_of_list_In.
-          destruct Ls.
-          + inversion Hsplit_sep as [[Heq Hnext]]; subst. 
-            destruct L; inversion Hnext as [[Heq Htail]]; subst.
-            - exfalso. 
-              pose proof (app_cons_not_nil Lm L2 succ).
-              congruence.
-            - by left.
-          + inversion Hsplit_sep as [[Heq Hnext]]; subst.
-            inversion Hcurr as [Heq]; subst.
-            apply in_app_iff; right; right.
-            rewrite app_ass -app_comm_cons in Hnext.
-            apply app_eq in Hnext.
-            destruct Lf; inversion Hnext as [[Heq Htail]]; subst.
-            - exfalso. 
-              pose proof (app_cons_not_nil Lm L2 succ).
-              congruence.
-            - by left.
-        }
-
-        iMod (own_update with "Hown_auth") as "[Hown_auth Hown_auth_frag']".
-        { apply auth_update_alloc, (gset_local_update_union _ _ {[ next ]}). }
-        assert (ε ∪ {[ next ]} = {[ next ]}) as -> by set_solver.
-        assert (S ∪ {[ next ]} = S) as -> by set_solver.
-
-        rewrite list_equiv_split; last first.
-        { rewrite app_ass -Hsplit_sep //. }
-        iDestruct "Hlist" as (n) "(Hpt & #Hn & Himp)".
-
-        wp_load.
-        iPoseProof ("Himp" with "Hpt") as "Hlist".
-        iMod ("Hclose" with "[Hlist Hown_auth Hown_toks Hown_frac]") as "_".
-        { iNext; iExists M, S, L; by iFrame. }
-
-        iModIntro. wp_load. 
-        wp_let. wp_lam. wp_pures.
-        case_bool_decide as Hcase.
-        * exfalso.
-          assert (node_key next <= node_key pred); last by lia.
-
-          assert (In pred (next :: Lm)) as Hpred_in_m.
-          {
-            symmetry in Hsplit_sep.
-            rewrite Hsplit_sep //= in Hsort.
-            rewrite //= app_comm_cons in Hsplit_join.
-            rewrite //= app_comm_cons Hcurr app_ass Hsplit_join in Hsplit_sep.
-            apply sorted_node_lt_no_dup in Hsort.
-
-            destruct Lm as [|next' Lm] using rev_ind.
-            + left. eapply (no_dup_elem_unique (Ls ++ [curr]) L2 (Ls ++ L1) L2 succ).
-                { rewrite app_ass //=. }
-                rewrite app_ass //= app_ass //=.
-            + right. apply in_app_iff. right. left.
-                eapply (no_dup_elem_unique (Ls ++ [curr; next] ++ Lm) L2 (Ls ++ L1) L2 succ).
-                { rewrite app_ass //= in Hsort. rewrite app_ass //=. }
-                rewrite app_ass //= in Hsplit_sep.
-                rewrite //= app_ass app_ass //=.
-          }
-
-          rewrite -Hsplit_sep in Hsort.
-          do 2 apply node_rep_sorted_app in Hsort as (_ & Hsort).
-          apply node_rep_sorted_app in Hsort as (Hsort & _).
-
-          apply Sorted_StronglySorted in Hsort; last first.
-          { unfold Relations_1.Transitive; apply node_lt_transitive. } 
-          inversion Hsort; subst. 
-          inversion Hpred_in_m; first by (subst; lia).
-          eapply node_lt_le_incl, Forall_forall; eauto.
-          rewrite elem_of_list_In //=.
-        * wp_if.
-          iApply ("IH" $! next with "[$] [$] [%]").
-          { lia. }
-          iNext; iApply "HΦ".
-    Qed.
-    
-    Theorem find_sub_spec (k lvl: Z) (head curr: node_rep)
-      (obot: option bot_gname) (sub: sub_gname) (osub: option sub_gname) :
-      {{{ 
-        inv (levelN lvl) (lazy_list_inv lvl head obot sub osub)
-        ∗
-        (⌜ curr = head ⌝ ∨ own (s_auth sub) (◯ {[ curr ]}))
-        ∗
-        ⌜ node_key curr < k < INT_MAX ⌝
-      }}}
-        find (rep_to_node curr) #k #lvl
-      {{{ pred succ, RET ((rep_to_node pred), (rep_to_node succ));
         ⌜ node_key pred < k ≤ node_key succ ⌝
         ∗
-        (⌜ pred = head ⌝ ∨ own (s_auth sub) (◯ {[ pred ]}))
-        ∗
-        (own (s_auth sub) (◯ {[ succ ]}) ∨ ⌜ succ = tail ⌝)
-        ∗
-        ∃ (γ: gname) (l: val), 
-          (node_locks pred +ₗ lvl) ↦□ l
-          ∗
-          is_lock γ l (in_lock lvl osub pred)
-      }}}.
+        has_lock lvl pred,
+      RET ((rep_to_node pred), (rep_to_node succ)) >>>.
     Proof.
-      iIntros (Φ) "(#Hinv & Hown_curr & Hrange) HΦ".
-      iRevert (curr) "Hown_curr Hrange HΦ".
-      iLöb as "IH".
-      iIntros (curr) "#Hown_curr %Hrange HΦ".
-      wp_lam. wp_pures. 
-      wp_lam. wp_pures.
+      iIntros "%Hk %Hlvl Hcurr #Hinv %Φ"; iRevert (curr Hk) "Hcurr".
+      iLöb as "IH"; iIntros "%curr %Hk #Hcurr AU".
+      wp_lam. wp_let. wp_let. wp_lam. wp_pures.
 
-      wp_bind (Load #(node_next curr +ₗ lvl)).
-      iInv (levelN lvl) as (M S L) "(Hinv_sub & Hmatch)" "Hclose".
-      iDestruct "Hinv_sub" as "(>%Hperm & >%Hsort & >Hown_auth & >Hown_toks & Hlist)".
+      wp_bind (Load #(node_next curr +ₗ lvl)). iInv "Hinv" as "Hskip". 
+      iDestruct (has_lvl_inv with "Hskip") as "(Hlvl & Hskip)"; first done.
+      iDestruct "Hlvl" as (S) "(>Hauth & >Hdisj & >Htoks & Hlocks & Hnexts & Hmap)".
 
-      iMod (own_update with "Hown_auth") as "[Hown_auth Hown_frag]".
-      { by apply auth_update_alloc, (gset_local_update S _ S). }
+      iDestruct (singleton_frag_in with "Hauth Hcurr") as %Hcurr.
+      rewrite (big_sepS_delete (has_lock _)) // (big_sepS_delete (has_next _ _)) //.
+      iDestruct "Hlocks" as "(#Hlock & Hlocks)"; iDestruct "Hnexts" as "(Hnext & Hnexts)".
+      iDestruct "Hnext" as (s succ) ">(Hnext & #Hs & #Hsucc & Hkeys)".
 
-      iAssert ((⌜ curr = head ∨ In curr L ⌝)%I) with "[Hown_auth Hown_curr]" as %Hcurr_range.
-      {
-        iDestruct "Hown_curr" as "[Heq|Hown]"; first by iLeft.
-        iDestruct (own_valid_2 with "Hown_auth Hown") 
-          as %[Hvalid%gset_included]%auth_both_valid_discrete.
-        iPureIntro; right.
-        rewrite -elem_of_list_In Hperm elem_of_elements.
-        set_solver.
-      }
+      destruct (decide (k ≤ node_key succ)) as [|Hcase].
+      + iMod "AU" as (d) "[Hexcl◯ [_ Hclose]]".
+        iDestruct (own_valid_2 with "Hdisj Hkeys") as %[Hdisj _]%ZRange_disj.
+        iDestruct (singleton_frag_in with "Hauth Hsucc") as %Hsucc%elem_of_union.
+        rewrite elem_of_singleton in Hsucc.
 
-      rewrite list_equiv_invert; last done.
-      iDestruct "Hlist" as (γ l s succ) "(>%Hsucc_range & Hpt & #Hs & #Hl & #Hlock & Himp)".
-      rewrite -elem_of_list_In Hperm elem_of_elements in Hsucc_range.
+        wp_load.
+        iAssert (has_next _ _ curr) with "[Hnext Hkeys]" as "Hnext".
+        { iExists s, succ; iFrame "# ∗". }
+        iCombine "Hlock Hlocks" as "Hlocks"; iCombine "Hnext Hnexts" as "Hnexts".
+        do 2 rewrite -big_sepS_delete //.
 
-      wp_load.
-      iPoseProof ("Himp" with "Hpt") as "Hlist".
-      iMod ("Hclose" with "[Hmatch Hlist Hown_auth Hown_toks]") as "_".
-      { iNext; iExists M, S, L; by iFrame. }
-
-      iModIntro. wp_load.
-      wp_let. wp_lam. wp_pures.
-      case_bool_decide as Hcase; wp_if.
-      - wp_pures. iApply "HΦ".
-        iModIntro; iFrame "#".
-
-        iSplit; first by (iPureIntro; lia).
-        iSplit.
+        iAssert ⌜ lvl = 0 → set_map node_key S = d ⌝%I with "[Hmap Hexcl◯]" as %Heqd.
         { 
-          destruct Hsucc_range as [Hin|Heq]; last by iRight.
-          assert (S = S ⋅ {[ succ ]}) as -> by set_solver.
-          iDestruct "Hown_frag" as "(? & ?)"; iLeft; iFrame.
+          iIntros (->); iDestruct "Hmap" as "(Hexcl● & _)".
+          by iDestruct (own_valid_2 with "Hexcl● Hexcl◯") as %<-%excl_auth_agree_L.
         }
-
-        iExists γ, l. iFrame "#".
-      - iApply ("IH" $! succ with "[Hown_frag] [%]").
+        iDestruct ("Hclose" with "[Hexcl◯]") as ">HΦ"; last iModIntro.
         {
-          iRight.
-          assert (S = S ⋅ {[ succ ]}) as ->.
-          {
-            destruct Hsucc_range as [Hin|Heq]; first set_solver.
-            subst; exfalso; rewrite /node_key/tail//= in Hcase; lia.
-          }
-          iDestruct "Hown_frag" as "(? & ?)"; iFrame.
+          iFrame "# ∗"; iPureIntro; split; last lia.
+          intros Hneq <-%Heqd Hfalse.
+          by apply (Hdisj k); last (rewrite zrange_spec; lia).
         }
-        { lia. }
 
-        iNext; iApply "HΦ".
+        iModIntro; iSplitR "HΦ".
+        { iNext; iApply "Hskip"; iExists S; iFrame. }
+        wp_load; wp_let; wp_lam; wp_pures.
+        case_bool_decide; last lia; wp_if.
+        by wp_pure.
+      + wp_load.
+        iAssert (has_next _ _ curr) with "[Hnext Hkeys]" as "Hnext".
+        { iExists s, succ; iFrame "# ∗". }
+        iCombine "Hlock Hlocks" as "Hlocks"; iCombine "Hnext Hnexts" as "Hnexts".
+        do 2 rewrite -big_sepS_delete //.
+
+        iModIntro; iSplitR "AU".
+        { iNext; iApply "Hskip"; iExists S; iFrame. }
+        wp_load; wp_let; wp_lam; wp_pures.
+        case_bool_decide; first lia; wp_if.
+        iDestruct "Hsucc" as "[->|Hsucc]"; first (rewrite /node_key/= in Hcase; lia).
+        iApply ("IH" with "[%] [$] AU"); lia.
     Qed.
 
-    Theorem findLock_spec (k lvl: Z) (head curr: node_rep)
-      (obot: option bot_gname) (sub: sub_gname) (osub: option sub_gname) :
-      {{{ 
-        inv (levelN lvl) (lazy_list_inv lvl head obot sub osub)
+    Theorem findLock_spec (k lvl: Z) (head curr: node_rep) (Γm: map_gname) (Γ: gmap Z inv_gname) :
+      node_key curr < k < INT_MAX →
+      0 ≤ lvl ≤ MAX_HEIGHT →
+      (⌜ curr = head ⌝ ∨ own (Γ !!! lvl).(auth_gname) (◯ {[curr]})) -∗
+      inv (skipN N) (skip_list_inv head Γm Γ) -∗
+      <<< ∀∀ (s: gset Z), own Γm.(excl_gname) (◯E s) >>>
+        findLock (rep_to_node curr) #k #lvl @ ↑(skipN N)
+      <<< ∃∃ pred succ,
+        own Γm.(excl_gname) (◯E s)
         ∗
-        (⌜ curr = head ⌝ ∨ own (s_auth sub) (◯ {[ curr ]}))
+        ⌜ k ≠ node_key succ → lvl = 0 → k ∉ s ⌝
         ∗
-        ⌜ node_key curr < k < INT_MAX ⌝
-      }}}
-        findLock (rep_to_node curr) #k #lvl
-      {{{ pred succ, RET ((rep_to_node pred), (rep_to_node succ));
+        (⌜ pred = head ⌝ ∨ own (Γ !!! lvl).(auth_gname) (◯ {[pred]}))
+        ∗
+        (⌜ succ = tail ⌝ ∨ own (Γ !!! lvl).(auth_gname) (◯ {[succ]}))
+        ∗
         ⌜ node_key pred < k ≤ node_key succ ⌝
         ∗
-        (⌜ pred = head ⌝ ∨ own (s_auth sub) (◯ {[ pred ]}))
-        ∗
-        (own (s_auth sub) (◯ {[ succ ]}) ∨ ⌜ succ = tail ⌝)
-        ∗
-        ∃ (γ: gname) (l: val) (s: loc), 
-          (node_locks pred +ₗ lvl) ↦□ l
+        ∃ (γl: gname) (l: val) (s: loc), 
+          (node_lock pred +ₗ lvl) ↦□ l
           ∗
-          is_lock γ l (in_lock lvl osub pred)
+          is_lock γl l (in_lock lvl (node_next pred))
           ∗
           (node_next pred +ₗ lvl) ↦{#1 / 2} #s
           ∗
           s ↦□ rep_to_node succ
           ∗
-          locked_val osub s
+          locked_val lvl s
           ∗
-          locked γ
-      }}}.
+          locked γl,
+      RET ((rep_to_node pred), (rep_to_node succ)) >>>.
     Proof.
-      iIntros (Φ) "(#Hinv & Hown_curr & Hrange) HΦ".
-      iRevert (curr) "Hown_curr Hrange".
-      iLöb as "IH". 
-      iIntros (curr) "#Hown_curr %Hrange".
+      iIntros "%Hk %Hlvl Hcurr #Hinv %Φ"; iRevert (curr Hk) "Hcurr".
+      iLöb as "IH"; iIntros (curr Hk) "#Hcurr AU".
+      wp_lam. wp_let. wp_let.
       
-      wp_lam. wp_pures.
-      wp_apply (find_sub_spec with "[Hown_curr]").
-      { by iFrame "#". }
-      iIntros (pred succ') "(%Hrange' & #Hown_pred & _ & Hlock)".
-      iDestruct "Hlock" as (γ l) "(#Hl & #Hlock)".
-      wp_pures. wp_lam. wp_pures.
+      awp_apply (find_spec with "Hcurr Hinv"); first done; first done.
+      iApply (aacc_aupd with "AU"); first done.
+      iIntros (d) "Hexcl◯"; iAaccIntro with "Hexcl◯".
+      { do 2 (iIntros "?"; iModIntro; iFrame). }
+      iIntros (pred succ') "(Hexcl◯ & _ & #Hpred & _ & (%Hk' & _) & Hlock)".
+      iDestruct "Hlock" as (γl l) "(#Hlock & #His_lock)".
 
-      wp_load. wp_let.
+      iModIntro; iLeft; iFrame. 
+      iIntros "AU"; iModIntro.
+      wp_pures; wp_lam; wp_pures; wp_load; wp_let.
+
       wp_bind (acquire _).
-      iApply (acquire_spec with "Hlock").
+      iApply (acquire_spec with "His_lock").
       iNext; iIntros "(Hlocked & Hin_lock)".
-      iDestruct "Hin_lock" as (s) "(Hnext & Hval)".
+      iDestruct "Hin_lock" as (s) "(Hnext' & Hval)".
+      wp_pures; wp_lam; wp_pures.
 
-      wp_pures. wp_lam. wp_pures.
-      wp_bind (Load #(node_next pred +ₗ lvl)).
-      iInv (levelN lvl) as (M S L) "(Hinv_sub & Hmatch)" "Hclose".
-      iDestruct "Hinv_sub" as "(>%Hperm & >%Hsort & >Hown_auth & >Hown_toks & Hlist)".
+      wp_bind (Load #(node_next pred +ₗ lvl)). iInv "Hinv" as "Hskip". 
+      iDestruct (has_lvl_inv with "Hskip") as "(Hlvl & Hskip)"; first done.
+      iDestruct "Hlvl" as (S) "(>Hauth & >Hdisj & >Htoks & Hlocks & Hnexts & Hmap)".
 
-      iMod (own_update with "Hown_auth") as "[Hown_auth Hown_frag]".
-      { by apply auth_update_alloc, (gset_local_update S _ S). }
+      iDestruct (singleton_frag_in with "Hauth Hpred") as %Hpred.
+      rewrite (big_sepS_delete (has_next _ _)) //.
+      iDestruct "Hnexts" as "(Hnext & Hnexts)".
+      iDestruct "Hnext" as (? succ) ">(Hnext & #Hs & #Hsucc & Hkeys)".
+      iDestruct (mapsto_agree with "Hnext Hnext'") as %Hs; inversion Hs; subst.
 
-      iAssert ⌜ pred = head ∨ In pred L ⌝%I
-        with "[Hown_auth Hown_pred]" as %Hpred_range.
-      {
-        iDestruct "Hown_pred" as "[Heq|Hown]"; first by iLeft.
-        iDestruct (own_valid_2 with "Hown_auth Hown") 
-          as %[Hvalid%gset_included]%auth_both_valid_discrete.
-        iPureIntro; right.
-        rewrite -elem_of_list_In Hperm elem_of_elements. 
-        set_solver.
-      }
+      destruct (decide (k ≤ node_key succ)) as [|Hcase].
+      + clear d; iMod "AU" as (d) "[Hexcl◯ [_ Hclose]]".
+        iDestruct (own_valid_2 with "Hdisj Hkeys") as %[Hdisj _]%ZRange_disj.
+        iDestruct (singleton_frag_in with "Hauth Hsucc") as %Hsucc%elem_of_union.
+        rewrite elem_of_singleton in Hsucc.
 
-      rewrite list_equiv_invert; last done.
-      iDestruct "Hlist" as (γ' l' s' succ) "(>%Hsucc_range & >Hpt & >#Hs' & _ & _ & Himp)".
-      rewrite -elem_of_list_In Hperm elem_of_elements in Hsucc_range.
-      iDestruct (mapsto_agree with "Hpt Hnext") as %Hs.
-      inversion Hs; subst.
+        wp_load.
+        iAssert (has_next _ _ pred) with "[Hnext Hkeys]" as "Hnext".
+        { iExists s, succ; iFrame "# ∗". }
+        iCombine "Hnext Hnexts" as "Hnexts".
+        rewrite -big_sepS_delete //.
 
-      iAssert (own (s_auth sub) (◯ {[succ]}) ∨ ⌜ succ = tail ⌝)%I
-        with "[Hown_frag]" as "#Hown_succ".
-      {
-        destruct Hsucc_range as [Hin|Heq]; last by iRight.
-        assert (S = S ⋅ {[ succ ]}) as -> by set_solver.
-        iDestruct "Hown_frag" as "(? & ?)"; iLeft; iFrame.
-      }
-
-      wp_load.
-      iPoseProof ("Himp" with "Hpt") as "Hlist".
-      iMod ("Hclose" with "[Hmatch Hlist Hown_auth Hown_toks]") as "_".
-      { iNext; iExists M, S, L; by iFrame. }
-
-      iModIntro. wp_load.
-      wp_let. wp_lam. wp_pures.
-      case_bool_decide as Hle; wp_if.
-      + wp_pures; iModIntro.
-        iApply "HΦ"; iFrame "# ∗".
-        iSplit; first by (iPureIntro; lia).
-        iExists γ, l, s. iFrame "# ∗".
-      + wp_apply (release_spec with "[Hnext Hval Hlocked]").
-        { iFrame "# ∗"; iExists s; iFrame. }
-        iIntros "_". wp_pures.
-
-        iApply ("IH" with "HΦ [] [%]").
-        {
-          iRight.
-          iDestruct "Hown_succ" as "[Hown|%Htail]"; first done.
-          rewrite Htail /node_key/tail/= in Hle; lia.
+        iAssert ⌜ lvl = 0 → set_map node_key S = d ⌝%I with "[Hmap Hexcl◯]" as %Heqd.
+        { 
+          iIntros (->); iDestruct "Hmap" as "(Hexcl● & _)".
+          by iDestruct (own_valid_2 with "Hexcl● Hexcl◯") as %<-%excl_auth_agree_L.
         }
-        { lia. }
-    Qed.
+        iDestruct ("Hclose" with "[Hexcl◯ Hlocked Hnext' Hval]") as ">HΦ"; last iModIntro.
+        {
+          iFrame "# ∗". iSplit. 
+          + iPureIntro; intros Hneq <-%Heqd Hfalse.
+            by apply (Hdisj k); last (rewrite zrange_spec; lia).
+          + iSplit; first (iPureIntro; lia). iExists γl, l, s; iFrame "# ∗".
+        }
 
-  End Proofs.
+        iModIntro; iSplitR "HΦ".
+        { iNext; iApply "Hskip"; iExists S; iFrame. }
+        wp_load; wp_let; wp_lam; wp_pures.
+        case_bool_decide; last lia; wp_if.
+        by wp_pure.
+      + wp_load.
+        iAssert (has_next _ _ pred) with "[Hnext Hkeys]" as "Hnext".
+        { iExists s, succ; iFrame "# ∗". }
+        iCombine "Hnext Hnexts" as "Hnexts".
+        rewrite -big_sepS_delete //.
+
+        iModIntro; iSplitR "AU Hlocked Hnext' Hval".
+        { iNext; iApply "Hskip"; iExists S; iFrame. }
+        wp_load; wp_let; wp_lam; wp_pures.
+        case_bool_decide; first lia; wp_if.
+        wp_apply (release_spec with "[Hlocked Hnext' Hval]").
+        { iFrame "# ∗"; iExists s; iFrame. }
+        iIntros "_"; wp_pures.
+        iDestruct "Hsucc" as "[->|Hsucc]"; first (rewrite /node_key/= in Hcase; lia).
+        iApply ("IH" with "[%] [$] AU"); lia.
+    Qed.
+  End proofs.
 End FindSpec.
