jelly_fish/spec/new.v
@@ -1,191 +1,154 @@
+From iris.algebra Require Import gmap gset excl_auth dfrac_agree.
 From iris.base_logic.lib Require Import invariants.
-From iris.algebra Require Import auth frac_auth gmap gset.
 From iris.heap_lang Require Import proofmode.
 
-From SkipList.lib Require Import arg_max.
-From SkipList.jelly_fish Require Import code.
-From SkipList.lib Require Import misc node_rep node_lt.
-From SkipList.jelly_fish.inv Require Import list_equiv lazy_inv skip_inv.
+From SkipList.lib Require Import zrange gmap_extra.
+From SkipList.jelly_fish Require Import code inv.
 
-
-Local Open Scope Z.
 
 Module NewSpec (Params: SKIP_LIST_PARAMS).
   Import Params.
   Module Invariant := SkipListInv Params.
   Export Invariant.
 
-  Section Proofs.
-    Context `{!heapGS Σ, !skipGS Σ, !lockG Σ}.
+  Section proofs.
+    Context `{!heapGS Σ, !skipG Σ} (N: namespace).
+    Local Open Scope Z.
 
     Theorem initLocks_spec (lvl: Z) (head: node_rep) (t: loc)
-      (bot: bot_gname) (subs: list sub_gname) :
+      (Γm: map_gname) (Γ: gmap Z inv_gname) :
+      1 ≤ lvl ≤ MAX_HEIGHT + 1 →
+      node_key head = INT_MIN →
+      t ↦□ rep_to_node tail -∗
       {{{
-        skip_list_equiv (lvl - 1) head ∅ 1 bot subs
-        ∗
-        t ↦□ rep_to_node tail
-        ∗
         (node_next head +ₗ lvl) ↦∗ replicate (Z.to_nat (MAX_HEIGHT + 1 - lvl)) #t
         ∗
-        (node_locks head +ₗ lvl) ↦∗ replicate (Z.to_nat (MAX_HEIGHT + 1 - lvl)) #()
+        (node_lock head +ₗ lvl) ↦∗ replicate (Z.to_nat (MAX_HEIGHT + 1 - lvl)) #()
         ∗
-        ⌜ 1 ≤ lvl ≤ MAX_HEIGHT + 1 ⌝ 
-        ∗
-        ⌜ node_key head = INT_MIN ⌝ 
+        [∗ set] i ∈ zrange (-1) lvl, lazy_list_inv head Γm Γ i
       }}}
-        initLocks #(node_locks head) #lvl
-      {{{ subs, RET #();
-        skip_list_equiv MAX_HEIGHT head ∅ 1 bot subs
-      }}}.
+        initLocks #(node_lock head) #lvl
+      {{{ Γ, RET #(); skip_list_inv head Γm Γ }}}.
     Proof.
-      iIntros (Φ) "(Hskip & #Ht & Hnext & Hlocks & Hlvl & %Hmin) HΦ".
-      iRevert (lvl subs) "Hskip Hnext Hlocks Hlvl HΦ".
+      iIntros "%Hlvl %Hmin #Ht %Φ !> (Hnexts & Hlocks & Hskip) HΦ".
+      iRevert (Γ lvl Hlvl) "Hnexts Hlocks Hskip HΦ".
       iLöb as "IH".
-      iIntros (lvl subs) "Hskip Hnext Hlocks %Hlvl HΦ".
+      iIntros (Γ lvl Hlvl) "Hnexts Hlocks Hskip HΦ".
 
       wp_lam. wp_let. wp_pures.
       case_bool_decide as Hcase; wp_if.
-      + iModIntro; iApply ("HΦ" $! subs).
-        inversion Hcase; subst.
-        by assert (MAX_HEIGHT + 1 - 1 = MAX_HEIGHT) as -> by lia.
+      + iModIntro; iApply ("HΦ" $! Γ).
+        inversion Hcase; subst; iFrame.
       + assert (lvl ≠ MAX_HEIGHT + 1) as Hneq by congruence.
-        destruct subs as [|γ subs]; first by iExFalso.
-
-        assert (Z.to_nat (MAX_HEIGHT + 1 - lvl) = S (Z.to_nat (MAX_HEIGHT - lvl))) as -> by lia.
+        replace (Z.to_nat (MAX_HEIGHT + 1 - lvl)) with (S (Z.to_nat (MAX_HEIGHT - lvl))) by lia.
         repeat rewrite replicate_S array_cons.
-        iDestruct "Hlocks" as "(Hl & Hlocks)".
-        iDestruct "Hnext" as "((Hnext' & Hnext'') & Hnext)".
+        iDestruct "Hlocks" as "(Hlock & Hlocks)".
+        iDestruct "Hnexts" as "((Hnext & Hnext') & Hnexts)".
 
-        wp_apply (newlock_spec (in_lock lvl (Some γ) head) with "[Hnext'']").
-        { iExists t; iFrame. }
-        iIntros (l γl) "#Hlock".
-
+        wp_apply (newlock_spec (in_lock lvl (node_next head)) with "[Hnext']").
+        { iExists t; iFrame; unfold locked_val; by case_decide; first lia. }
+        iIntros (l γl) "#His_lock".
         wp_store. wp_pures.
-        iMod (mapsto_persist with "Hl") as "#Hl".
+        iMod (mapsto_persist with "Hlock") as "#Hlock".
 
-        iMod (own_alloc (● ∅ ⋅ ◯ ∅))
-          as (γauth) "[Hown_auth _]"; 
+        iMod (own_alloc (● (∅ : gset node_rep) ⋅ ◯ ∅))
+          as (γauth) "[Hauth _]"; 
           first by apply auth_both_valid.
+        iMod (own_alloc (GSet ∅ ⋅ ZRange (node_key head) (node_key tail)))
+          as (γdisj) "[Hdisj Hkeys]";
+          first by (pose HMIN_MAX; rewrite Hmin ZRange_disj).
         iMod (own_alloc (● GSet ∅ ⋅ ◯ GSet ∅))
-          as (γtoks) "[Hown_toks _]"; 
+          as (γtoks) "[Htoks _]"; 
           first by apply auth_both_valid.
+        set (Γi := mk_inv_gname γauth γdisj γtoks).
+        set (Γ' := <[lvl := Γi]>Γ).
 
-        set (Γ := mk_sub_gname γauth γtoks).
-        iMod (inv_alloc (levelN lvl) ⊤ (lazy_list_inv lvl head None Γ (Some γ)) 
-          with "[Hnext' Hown_auth Hown_toks]") as "Hinv".
+        rewrite ?loc_add_assoc; replace (MAX_HEIGHT - lvl) with (MAX_HEIGHT + 1 - (lvl + 1)) by lia.
+        iApply ("IH" $! Γ' with "[%] Hnexts Hlocks [-HΦ]"); first lia.
         {
-          iNext; iExists ∅, ∅, nil.
-          rewrite /sub_list_inv set_map_empty.
-          iFrame. iSplit; first done. 
-          iSplit.
-          {
-            assert (node_lt head tail); last (simpl; auto).
-            rewrite /node_key in Hmin.
-            rewrite /node_lt /node_key Hmin /=; apply HMIN_MAX.
-          }
-          iExists γl, l, t; iFrame "# ∗".
+          rewrite (zrange_split_r _ lvl); last lia.
+          rewrite comm_L big_sepS_insert; last (rewrite zrange_spec; lia).
+          iSplitR "Hskip".
+          + iExists ∅; case_decide; first lia.
+            rewrite right_id_L ?big_sepS_singleton big_sepS_empty set_map_empty lookup_total_insert; iFrame.
+            iSplit; first (iExists γl, l; iFrame "#").
+            iSplit; last done. iExists t, tail; iFrame "# ∗"; by iLeft.
+          + iApply big_sepS_mono; last iFrame.
+            iIntros (m Hm%zrange_spec) "Hlvl".
+            rewrite /lazy_list_inv ?lookup_total_insert_ne //; lia.
         }
-
-        iApply ("IH" $! _ (Γ :: γ :: subs) with "[Hskip Hinv] [Hnext] [Hlocks] [%]").
-        {
-          assert (lvl + 1 - 1 = lvl) as -> by lia.
-          iFrame. iPureIntro; lia.
-        }
-        {
-          assert (MAX_HEIGHT + 1 - (lvl + 1) = MAX_HEIGHT - lvl) as -> by lia.
-          rewrite -loc_add_assoc //.
-        }
-        {
-          assert (MAX_HEIGHT + 1 - (lvl + 1) = MAX_HEIGHT - lvl) as -> by lia.
-          rewrite -loc_add_assoc //.
-        }
-        { lia. }
-
         iNext; done.
     Qed.
 
     Theorem new_spec : 
       {{{ True }}}
         new #()
-      {{{ p bot subs, RET #p; is_skip_list p ∅ 1 bot subs }}}.
+      {{{ p Γm, RET #p; map_inv N p Γm ∗ map ∅ Γm }}}.
     Proof.
-      iIntros (Φ) "_ HΦ".
-      pose proof HMAX_HEIGHT as Hmax.
+      iIntros (Φ) "_ HΦ"; wp_lam; pose proof HMAX_HEIGHT. 
 
-      wp_lam. 
       wp_alloc t as "Ht"; iMod (mapsto_persist with "Ht") as "#Ht".
-      wp_alloc next as "Hnext"; first lia. wp_let.
+      wp_alloc next as "Hnexts"; first lia. wp_let.
       wp_alloc locks as "Hlocks"; first lia. wp_let.
 
-      assert (Z.to_nat (MAX_HEIGHT + 1) = S (Z.to_nat MAX_HEIGHT)) as -> by lia.
+      replace (Z.to_nat (MAX_HEIGHT + 1)) with (S (Z.to_nat MAX_HEIGHT)) by lia.
       rewrite replicate_S ?array_cons.
-      iDestruct "Hnext" as "((Hn & Hn') & Hnext)".
-      iDestruct "Hlocks" as "(Hlocks' & Hlocks)".
+      iDestruct "Hnexts" as "((Hnext & Hnext') & Hnexts)".
+      iDestruct "Hlocks" as "(Hlock & Hlocks)".
 
       wp_lam. wp_let. wp_pures.
       case_bool_decide as Hcase; first (inversion Hcase; lia).
       wp_if.
 
-      set (head := (INT_MIN, dummy_null, next, @None loc, dummy_lock, locks)).
-      wp_apply (newlock_spec (in_lock 0 None head) with "[Hn']").
-      { 
-        iExists t; rewrite loc_add_0; iFrame.
-        iExists tail; iFrame "#"; by iLeft.
-      }
-      iIntros (l γl) "#Hlock".
+      iMod (own_alloc (●E ∅ ⋅ ◯E ∅))
+        as (γexcl) "[Hexcl● Hexcl◯]";
+        first by apply auth_both_valid.
+      iMod (own_alloc (● DMap ∅ ⋅ ◯ DMap∅))
+        as (γvals) "[Hvals _]"; 
+        first by apply auth_both_valid.
+      set (Γm := mk_map_gname γexcl γvals).
+      set (head := (INT_MIN, dummy_null, next, locks)).
+      wp_apply (newlock_spec (in_lock 0 (node_next head)) with "[Hnext']").
+      { iExists t; rewrite loc_add_0; iFrame. iExists tail; iFrame "#"; by iLeft. }
+      iIntros (l γl) "#His_lock".
 
       wp_pures; rewrite loc_add_0.
-      wp_store; iMod (mapsto_persist with "Hlocks'") as "#Hl".
-      wp_pures; assert (0 + 1 = 1) as -> by lia.
+      wp_store; iMod (mapsto_persist with "Hlock") as "#Hlock".
+      wp_pures; replace (0 + 1) with 1 by lia.
 
       iMod (own_alloc (● ∅ ⋅ ◯ ∅))
-        as (γauth) "[Hown_auth _]"; 
+        as (γauth) "[Hauth _]"; 
         first by apply auth_both_valid.
+      iMod (own_alloc (GSet ∅ ⋅ ZRange (node_key head) (node_key tail)))
+        as (γdisj) "[Hdisj Hkeys]";
+        first by (pose HMIN_MAX; rewrite ZRange_disj).
       iMod (own_alloc (● GSet ∅ ⋅ ◯ GSet ∅))
-        as (γtoks) "[Hown_toks _]"; 
+        as (γtoks) "[Htoks _]"; 
         first by apply auth_both_valid.
-      iMod (own_alloc (●F (∅ : gmap Z (argmax Z)) ⋅ ◯F (∅: gmap Z (argmax Z))))
-        as (γfrac) "[Hown_frac Hown_frac_frag]"; 
-        first by apply auth_both_valid.
+      set (Γi := mk_inv_gname γauth γdisj γtoks).
+      set (Γ' := ({[ 0 := Γi ]} : gmap Z inv_gname)).
 
-      set (Γ := mk_sub_gname γauth γtoks).
-      set (bot := mk_bot_gname γfrac).
-      iMod (inv_alloc (levelN 0) ⊤ (lazy_list_inv 0 head (Some bot) Γ None) 
-        with "[Hn Hown_auth Hown_toks Hown_frac]") as "Hinv".
+      replace locks with (node_lock head) by auto.
+      replace Γi with (Γ' !!! 0) by set_solver.
+      wp_apply (initLocks_spec _ _ _ Γm Γ' with "Ht [-HΦ Hexcl◯ Hvals]"); first lia; first done.
       {
-        iNext; iExists ∅, ∅, nil. 
-        rewrite /sub_list_inv set_map_empty dom_empty_L.
-        iFrame. iSplit; last done. iSplit; first done. 
-        iSplit.
-        {
-          assert (node_lt head tail); last (simpl; auto).
-          rewrite /node_lt/node_key//=; apply HMIN_MAX.
-        }
-
-        iExists γl, l, t.
-        repeat rewrite loc_add_0.
-        iFrame "# ∗".
+        replace (MAX_HEIGHT + 1 - 1) with MAX_HEIGHT by lia; iFrame. 
+        replace 1 with (0 + 1) by lia; rewrite zrange_split_r; last lia.
+        replace 0 with (-1 + 1) by lia; rewrite zrange_empty_r left_id_L big_sepS_singleton //.
+        iExists ∅; case_decide; last lia.
+        replace (Γ' !!! 0) with Γi by set_solver.
+        rewrite right_id_L ?big_sepS_singleton /own_map big_sepS_empty set_map_empty; iFrame. 
+        iSplit; first (iExists γl, l; rewrite ?loc_add_0; iFrame "#").
+        iExists t, tail; rewrite loc_add_0; iFrame "# ∗"; by iLeft.
       }
+      iIntros (Γ) "Hskip".
+      iMod (inv_alloc (skipN N) ⊤ (skip_list_inv head Γm Γ) with "Hskip") as "#Hinv".
 
-      iAssert (skip_list_equiv 0 head ∅ 1 bot [Γ]) 
-        with "[Hinv Hown_frac_frag]" as "Hskip".
-      { by iFrame. }
-
-      assert (locks = node_locks head) as Hlocks by auto; rewrite Hlocks.
-      wp_apply (initLocks_spec 1 head t with "[Hskip Hlocks Hnext]").
-      {
-        assert (MAX_HEIGHT + 1 - 1 = MAX_HEIGHT) as -> by lia.
-        assert (1 - 1 = 0) as -> by lia.
-        iFrame "# ∗". iPureIntro.
-        by split; first lia.
-      }
-      iIntros (subs) "Hskip". wp_pures.
-      rewrite (fold_rep_to_node head).
-
+      wp_pures; rewrite (fold_rep_to_node head).
       wp_alloc p as "Hp"; iMod (mapsto_persist with "Hp") as "#Hp".
-      iModIntro; iApply ("HΦ" $! p bot subs).
-      iExists head. by iFrame "# ∗".
+      iModIntro; iApply ("HΦ" $! _ Γm).
+      iSplit; first by (iExists head, Γ; iFrame "#").
+      rewrite -dom_empty; iFrame.
     Qed.
-
-  End Proofs.
+  End proofs.
 End NewSpec.
